# Note
```
guid: ok{j3gQ=I(
notetype: Basic
```

### Tags
```
```

## Front
Vergleichssatz

## Back
Seien \(\sum\limits_{k=1}^\infty a_k\) und \(\sum\limits_{k=1}^\infty b_k\) Reihen so, dass gilt \(\forall k:0\leq a_k\leq b_k\) dann gilt:
\(\sum\limits_{k=1}^\infty b_k\text{ konvergent}\implies\sum\limits_{k=1}^\infty a_k \text{ konvergent}\)
\(\sum\limits_{k=1}^\infty a_k\text{ divergent}\implies\sum\limits_{k=1}^\infty b_k \text{ divergent}\)

diese Implikationen treffen auch mit der bedingung \(K\geq 1, \forall k\geq K:0\leq a_k\leq b_k\) zu.
